examples/ghc/lib/OrdList.v
@@ -51,7 +51,7 @@ Arguments Two {_} _ _.
 (* Skipping all instances of class `Outputable.Outputable', including
    `OrdList.Outputable__OrdList' *)
 
-Definition appOL {a} : OrdList a -> OrdList a -> OrdList a :=
+Definition appOL {a : Type} : OrdList a -> OrdList a -> OrdList a :=
   fun arg_0__ arg_1__ =>
     match arg_0__, arg_1__ with
     | None, b => b
@@ -61,38 +61,40 @@ Definition appOL {a} : OrdList a -> OrdList a -> OrdList a :=
     | a, b => Two a b
     end.
 
-Local Definition Semigroup__OrdList_op_zlzlzgzg__ {inst_a}
-   : (OrdList inst_a) -> (OrdList inst_a) -> (OrdList inst_a) :=
+Local Definition Semigroup__OrdList_op_zlzlzgzg__ {inst_a : Type}
+   : OrdList inst_a -> OrdList inst_a -> OrdList inst_a :=
   appOL.
 
-Program Instance Semigroup__OrdList {a} : GHC.Base.Semigroup (OrdList a) :=
+Program Instance Semigroup__OrdList {a : Type}
+   : GHC.Base.Semigroup (OrdList a) :=
   fun _ k__ =>
     k__ {| GHC.Base.op_zlzlzgzg____ := Semigroup__OrdList_op_zlzlzgzg__ |}.
 
-Local Definition Monoid__OrdList_mappend {inst_a}
-   : (OrdList inst_a) -> (OrdList inst_a) -> (OrdList inst_a) :=
+Local Definition Monoid__OrdList_mappend {inst_a : Type}
+   : OrdList inst_a -> OrdList inst_a -> OrdList inst_a :=
   _GHC.Base.<<>>_.
 
-Definition concatOL {a} : list (OrdList a) -> OrdList a :=
+Definition concatOL {a : Type} : list (OrdList a) -> OrdList a :=
   fun aas => Data.Foldable.foldr appOL None aas.
 
-Local Definition Monoid__OrdList_mconcat {inst_a}
-   : list (OrdList inst_a) -> (OrdList inst_a) :=
+Local Definition Monoid__OrdList_mconcat {inst_a : Type}
+   : list (OrdList inst_a) -> OrdList inst_a :=
   concatOL.
 
-Definition nilOL {a} : OrdList a :=
+Definition nilOL {a : Type} : OrdList a :=
   None.
 
-Local Definition Monoid__OrdList_mempty {inst_a} : (OrdList inst_a) :=
+Local Definition Monoid__OrdList_mempty {inst_a : Type} : OrdList inst_a :=
   nilOL.
 
-Program Instance Monoid__OrdList {a} : GHC.Base.Monoid (OrdList a) :=
+Program Instance Monoid__OrdList {a : Type} : GHC.Base.Monoid (OrdList a) :=
   fun _ k__ =>
     k__ {| GHC.Base.mappend__ := Monoid__OrdList_mappend ;
            GHC.Base.mconcat__ := Monoid__OrdList_mconcat ;
            GHC.Base.mempty__ := Monoid__OrdList_mempty |}.
 
-Fixpoint mapOL {a} {b} (arg_0__ : (a -> b)) (arg_1__ : OrdList a) : OrdList b
+Fixpoint mapOL {a : Type} {b : Type} (arg_0__ : a -> b) (arg_1__ : OrdList a)
+  : OrdList b
   := match arg_0__, arg_1__ with
      | _, None => None
      | f, One x => One (f x)
@@ -103,20 +105,21 @@ Fixpoint mapOL {a} {b} (arg_0__ : (a -> b)) (arg_1__ : OrdList a) : OrdList b
      end.
 
 Local Definition Functor__OrdList_fmap
-   : forall {a} {b}, (a -> b) -> OrdList a -> OrdList b :=
-  fun {a} {b} => mapOL.
+   : forall {a : Type}, forall {b : Type}, (a -> b) -> OrdList a -> OrdList b :=
+  fun {a : Type} {b : Type} => mapOL.
 
 Local Definition Functor__OrdList_op_zlzd__
-   : forall {a} {b}, a -> OrdList b -> OrdList a :=
-  fun {a} {b} => Functor__OrdList_fmap GHC.Base.∘ GHC.Base.const.
+   : forall {a : Type}, forall {b : Type}, a -> OrdList b -> OrdList a :=
+  fun {a : Type} {b : Type} => Functor__OrdList_fmap GHC.Base.∘ GHC.Base.const.
 
 Program Instance Functor__OrdList : GHC.Base.Functor OrdList :=
   fun _ k__ =>
-    k__ {| GHC.Base.fmap__ := fun {a} {b} => Functor__OrdList_fmap ;
-           GHC.Base.op_zlzd____ := fun {a} {b} => Functor__OrdList_op_zlzd__ |}.
+    k__ {| GHC.Base.fmap__ := fun {a : Type} {b : Type} => Functor__OrdList_fmap ;
+           GHC.Base.op_zlzd____ := fun {a : Type} {b : Type} =>
+             Functor__OrdList_op_zlzd__ |}.
 
-Fixpoint foldrOL {a} {b} (arg_0__ : (a -> b -> b)) (arg_1__ : b) (arg_2__
-                   : OrdList a) : b
+Fixpoint foldrOL {a : Type} {b : Type} (arg_0__ : a -> b -> b) (arg_1__ : b)
+                 (arg_2__ : OrdList a) : b
   := match arg_0__, arg_1__, arg_2__ with
      | _, z, None => z
      | k, z, One x => k x z
@@ -127,22 +130,23 @@ Fixpoint foldrOL {a} {b} (arg_0__ : (a -> b -> b)) (arg_1__ : b) (arg_2__
      end.
 
 Local Definition Foldable__OrdList_foldr
-   : forall {a} {b}, (a -> b -> b) -> b -> OrdList a -> b :=
-  fun {a} {b} => foldrOL.
+   : forall {a : Type}, forall {b : Type}, (a -> b -> b) -> b -> OrdList a -> b :=
+  fun {a : Type} {b : Type} => foldrOL.
 
 Local Definition Foldable__OrdList_foldMap
-   : forall {m} {a}, forall `{GHC.Base.Monoid m}, (a -> m) -> OrdList a -> m :=
-  fun {m} {a} `{GHC.Base.Monoid m} =>
+   : forall {m : Type},
+     forall {a : Type}, forall `{GHC.Base.Monoid m}, (a -> m) -> OrdList a -> m :=
+  fun {m : Type} {a : Type} `{GHC.Base.Monoid m} =>
     fun f =>
       Foldable__OrdList_foldr (GHC.Base.mappend GHC.Base.∘ f) GHC.Base.mempty.
 
 Local Definition Foldable__OrdList_fold
-   : forall {m}, forall `{GHC.Base.Monoid m}, OrdList m -> m :=
-  fun {m} `{GHC.Base.Monoid m} => Foldable__OrdList_foldMap GHC.Base.id.
+   : forall {m : Type}, forall `{GHC.Base.Monoid m}, OrdList m -> m :=
+  fun {m : Type} `{GHC.Base.Monoid m} => Foldable__OrdList_foldMap GHC.Base.id.
 
 Local Definition Foldable__OrdList_foldl
-   : forall {b} {a}, (b -> a -> b) -> b -> OrdList a -> b :=
-  fun {b} {a} =>
+   : forall {b : Type}, forall {a : Type}, (b -> a -> b) -> b -> OrdList a -> b :=
+  fun {b : Type} {a : Type} =>
     fun f z t =>
       Data.SemigroupInternal.appEndo (Data.SemigroupInternal.getDual
                                       (Foldable__OrdList_foldMap (Data.SemigroupInternal.Mk_Dual GHC.Base.∘
@@ -150,64 +154,69 @@ Local Definition Foldable__OrdList_foldl
                                                                    GHC.Base.flip f)) t)) z.
 
 Local Definition Foldable__OrdList_foldl'
-   : forall {b} {a}, (b -> a -> b) -> b -> OrdList a -> b :=
-  fun {b} {a} =>
+   : forall {b : Type}, forall {a : Type}, (b -> a -> b) -> b -> OrdList a -> b :=
+  fun {b : Type} {a : Type} =>
     fun f z0 xs =>
       let f' := fun x k z => k (f z x) in
       Foldable__OrdList_foldr f' GHC.Base.id xs z0.
 
 Local Definition Foldable__OrdList_foldr'
-   : forall {a} {b}, (a -> b -> b) -> b -> OrdList a -> b :=
-  fun {a} {b} =>
+   : forall {a : Type}, forall {b : Type}, (a -> b -> b) -> b -> OrdList a -> b :=
+  fun {a : Type} {b : Type} =>
     fun f z0 xs =>
       let f' := fun k x z => k (f x z) in
       Foldable__OrdList_foldl f' GHC.Base.id xs z0.
 
 Local Definition Foldable__OrdList_length
-   : forall {a}, OrdList a -> GHC.Num.Int :=
-  fun {a} =>
+   : forall {a : Type}, OrdList a -> GHC.Num.Int :=
+  fun {a : Type} =>
     Foldable__OrdList_foldl' (fun arg_0__ arg_1__ =>
                                 match arg_0__, arg_1__ with
                                 | c, _ => c GHC.Num.+ #1
                                 end) #0.
 
-Local Definition Foldable__OrdList_null : forall {a}, OrdList a -> bool :=
-  fun {a} => Foldable__OrdList_foldr (fun arg_0__ arg_1__ => false) true.
+Local Definition Foldable__OrdList_null
+   : forall {a : Type}, OrdList a -> bool :=
+  fun {a : Type} => Foldable__OrdList_foldr (fun arg_0__ arg_1__ => false) true.
 
 Local Definition Foldable__OrdList_product
-   : forall {a}, forall `{GHC.Num.Num a}, OrdList a -> a :=
-  fun {a} `{GHC.Num.Num a} =>
+   : forall {a : Type}, forall `{GHC.Num.Num a}, OrdList a -> a :=
+  fun {a : Type} `{GHC.Num.Num a} =>
     Coq.Program.Basics.compose Data.SemigroupInternal.getProduct
                                (Foldable__OrdList_foldMap Data.SemigroupInternal.Mk_Product).
 
 Local Definition Foldable__OrdList_sum
-   : forall {a}, forall `{GHC.Num.Num a}, OrdList a -> a :=
-  fun {a} `{GHC.Num.Num a} =>
+   : forall {a : Type}, forall `{GHC.Num.Num a}, OrdList a -> a :=
+  fun {a : Type} `{GHC.Num.Num a} =>
     Coq.Program.Basics.compose Data.SemigroupInternal.getSum
                                (Foldable__OrdList_foldMap Data.SemigroupInternal.Mk_Sum).
 
-Local Definition Foldable__OrdList_toList : forall {a}, OrdList a -> list a :=
-  fun {a} =>
+Local Definition Foldable__OrdList_toList
+   : forall {a : Type}, OrdList a -> list a :=
+  fun {a : Type} =>
     fun t => GHC.Base.build' (fun _ => (fun c n => Foldable__OrdList_foldr c n t)).
 
 Program Instance Foldable__OrdList : Data.Foldable.Foldable OrdList :=
   fun _ k__ =>
-    k__ {| Data.Foldable.fold__ := fun {m} `{GHC.Base.Monoid m} =>
+    k__ {| Data.Foldable.fold__ := fun {m : Type} `{GHC.Base.Monoid m} =>
              Foldable__OrdList_fold ;
-           Data.Foldable.foldMap__ := fun {m} {a} `{GHC.Base.Monoid m} =>
+           Data.Foldable.foldMap__ := fun {m : Type} {a : Type} `{GHC.Base.Monoid m} =>
              Foldable__OrdList_foldMap ;
-           Data.Foldable.foldl__ := fun {b} {a} => Foldable__OrdList_foldl ;
-           Data.Foldable.foldl'__ := fun {b} {a} => Foldable__OrdList_foldl' ;
-           Data.Foldable.foldr__ := fun {a} {b} => Foldable__OrdList_foldr ;
-           Data.Foldable.foldr'__ := fun {a} {b} => Foldable__OrdList_foldr' ;
-           Data.Foldable.length__ := fun {a} => Foldable__OrdList_length ;
-           Data.Foldable.null__ := fun {a} => Foldable__OrdList_null ;
-           Data.Foldable.product__ := fun {a} `{GHC.Num.Num a} =>
+           Data.Foldable.foldl__ := fun {b : Type} {a : Type} => Foldable__OrdList_foldl ;
+           Data.Foldable.foldl'__ := fun {b : Type} {a : Type} =>
+             Foldable__OrdList_foldl' ;
+           Data.Foldable.foldr__ := fun {a : Type} {b : Type} => Foldable__OrdList_foldr ;
+           Data.Foldable.foldr'__ := fun {a : Type} {b : Type} =>
+             Foldable__OrdList_foldr' ;
+           Data.Foldable.length__ := fun {a : Type} => Foldable__OrdList_length ;
+           Data.Foldable.null__ := fun {a : Type} => Foldable__OrdList_null ;
+           Data.Foldable.product__ := fun {a : Type} `{GHC.Num.Num a} =>
              Foldable__OrdList_product ;
-           Data.Foldable.sum__ := fun {a} `{GHC.Num.Num a} => Foldable__OrdList_sum ;
-           Data.Foldable.toList__ := fun {a} => Foldable__OrdList_toList |}.
+           Data.Foldable.sum__ := fun {a : Type} `{GHC.Num.Num a} =>
+             Foldable__OrdList_sum ;
+           Data.Foldable.toList__ := fun {a : Type} => Foldable__OrdList_toList |}.
 
-Definition fromOL {a} : OrdList a -> list a :=
+Definition fromOL {a : Type} : OrdList a -> list a :=
   fun a =>
     let fix go arg_0__ arg_1__
       := match arg_0__, arg_1__ with
@@ -220,57 +229,75 @@ Definition fromOL {a} : OrdList a -> list a :=
          end in
     go a nil.
 
-Definition toOL {a} : list a -> OrdList a :=
+Definition toOL {a : Type} : list a -> OrdList a :=
   fun arg_0__ => match arg_0__ with | nil => None | xs => Many xs end.
 
 Local Definition Traversable__OrdList_traverse
-   : forall {f} {a} {b},
+   : forall {f : Type -> Type},
+     forall {a : Type},
+     forall {b : Type},
      forall `{GHC.Base.Applicative f}, (a -> f b) -> OrdList a -> f (OrdList b) :=
-  fun {f} {a} {b} `{GHC.Base.Applicative f} =>
+  fun {f : Type -> Type} {a : Type} {b : Type} `{GHC.Base.Applicative f} =>
     fun f xs => toOL Data.Functor.<$> Data.Traversable.traverse f (fromOL xs).
 
 Local Definition Traversable__OrdList_mapM
-   : forall {m} {a} {b},
+   : forall {m : Type -> Type},
+     forall {a : Type},
+     forall {b : Type},
      forall `{GHC.Base.Monad m}, (a -> m b) -> OrdList a -> m (OrdList b) :=
-  fun {m} {a} {b} `{GHC.Base.Monad m} => Traversable__OrdList_traverse.
+  fun {m : Type -> Type} {a : Type} {b : Type} `{GHC.Base.Monad m} =>
+    Traversable__OrdList_traverse.
 
 Local Definition Traversable__OrdList_sequenceA
-   : forall {f} {a},
+   : forall {f : Type -> Type},
+     forall {a : Type},
      forall `{GHC.Base.Applicative f}, OrdList (f a) -> f (OrdList a) :=
-  fun {f} {a} `{GHC.Base.Applicative f} =>
+  fun {f : Type -> Type} {a : Type} `{GHC.Base.Applicative f} =>
     Traversable__OrdList_traverse GHC.Base.id.
 
 Local Definition Traversable__OrdList_sequence
-   : forall {m} {a}, forall `{GHC.Base.Monad m}, OrdList (m a) -> m (OrdList a) :=
-  fun {m} {a} `{GHC.Base.Monad m} => Traversable__OrdList_sequenceA.
+   : forall {m : Type -> Type},
+     forall {a : Type}, forall `{GHC.Base.Monad m}, OrdList (m a) -> m (OrdList a) :=
+  fun {m : Type -> Type} {a : Type} `{GHC.Base.Monad m} =>
+    Traversable__OrdList_sequenceA.
 
 Program Instance Traversable__OrdList : Data.Traversable.Traversable OrdList :=
   fun _ k__ =>
-    k__ {| Data.Traversable.mapM__ := fun {m} {a} {b} `{GHC.Base.Monad m} =>
+    k__ {| Data.Traversable.mapM__ := fun {m : Type -> Type}
+           {a : Type}
+           {b : Type}
+           `{GHC.Base.Monad m} =>
              Traversable__OrdList_mapM ;
-           Data.Traversable.sequence__ := fun {m} {a} `{GHC.Base.Monad m} =>
+           Data.Traversable.sequence__ := fun {m : Type -> Type}
+           {a : Type}
+           `{GHC.Base.Monad m} =>
              Traversable__OrdList_sequence ;
-           Data.Traversable.sequenceA__ := fun {f} {a} `{GHC.Base.Applicative f} =>
+           Data.Traversable.sequenceA__ := fun {f : Type -> Type}
+           {a : Type}
+           `{GHC.Base.Applicative f} =>
              Traversable__OrdList_sequenceA ;
-           Data.Traversable.traverse__ := fun {f} {a} {b} `{GHC.Base.Applicative f} =>
+           Data.Traversable.traverse__ := fun {f : Type -> Type}
+           {a : Type}
+           {b : Type}
+           `{GHC.Base.Applicative f} =>
              Traversable__OrdList_traverse |}.
 
-Definition unitOL {a} : a -> OrdList a :=
+Definition unitOL {a : Type} : a -> OrdList a :=
   fun as_ => One as_.
 
-Definition snocOL {a} : OrdList a -> a -> OrdList a :=
+Definition snocOL {a : Type} : OrdList a -> a -> OrdList a :=
   fun as_ b => Snoc as_ b.
 
-Definition consOL {a} : a -> OrdList a -> OrdList a :=
+Definition consOL {a : Type} : a -> OrdList a -> OrdList a :=
   fun a bs => Cons a bs.
 
 (* Skipping definition `OrdList.lastOL' *)
 
-Definition isNilOL {a} : OrdList a -> bool :=
+Definition isNilOL {a : Type} : OrdList a -> bool :=
   fun arg_0__ => match arg_0__ with | None => true | _ => false end.
 
-Fixpoint foldlOL {b} {a} (arg_0__ : (b -> a -> b)) (arg_1__ : b) (arg_2__
-                   : OrdList a) : b
+Fixpoint foldlOL {b : Type} {a : Type} (arg_0__ : b -> a -> b) (arg_1__ : b)
+                 (arg_2__ : OrdList a) : b
   := match arg_0__, arg_1__, arg_2__ with
      | _, z, None => z
      | k, z, One x => k z x
@@ -281,18 +308,18 @@ Fixpoint foldlOL {b} {a} (arg_0__ : (b -> a -> b)) (arg_1__ : b) (arg_2__
      end.
 
 (* External variables:
-     bool cons false list nil true Coq.Init.Datatypes.app Coq.Program.Basics.compose
-     Data.Foldable.Foldable Data.Foldable.foldMap__ Data.Foldable.fold__
-     Data.Foldable.foldl Data.Foldable.foldl'__ Data.Foldable.foldl__
-     Data.Foldable.foldr Data.Foldable.foldr'__ Data.Foldable.foldr__
-     Data.Foldable.length__ Data.Foldable.null__ Data.Foldable.product__
-     Data.Foldable.sum__ Data.Foldable.toList__ Data.Functor.op_zlzdzg__
-     Data.SemigroupInternal.Mk_Dual Data.SemigroupInternal.Mk_Endo
-     Data.SemigroupInternal.Mk_Product Data.SemigroupInternal.Mk_Sum
-     Data.SemigroupInternal.appEndo Data.SemigroupInternal.getDual
-     Data.SemigroupInternal.getProduct Data.SemigroupInternal.getSum
-     Data.Traversable.Traversable Data.Traversable.mapM__
-     Data.Traversable.sequenceA__ Data.Traversable.sequence__
+     Type bool cons false list nil true Coq.Init.Datatypes.app
+     Coq.Program.Basics.compose Data.Foldable.Foldable Data.Foldable.foldMap__
+     Data.Foldable.fold__ Data.Foldable.foldl Data.Foldable.foldl'__
+     Data.Foldable.foldl__ Data.Foldable.foldr Data.Foldable.foldr'__
+     Data.Foldable.foldr__ Data.Foldable.length__ Data.Foldable.null__
+     Data.Foldable.product__ Data.Foldable.sum__ Data.Foldable.toList__
+     Data.Functor.op_zlzdzg__ Data.SemigroupInternal.Mk_Dual
+     Data.SemigroupInternal.Mk_Endo Data.SemigroupInternal.Mk_Product
+     Data.SemigroupInternal.Mk_Sum Data.SemigroupInternal.appEndo
+     Data.SemigroupInternal.getDual Data.SemigroupInternal.getProduct
+     Data.SemigroupInternal.getSum Data.Traversable.Traversable
+     Data.Traversable.mapM__ Data.Traversable.sequenceA__ Data.Traversable.sequence__
      Data.Traversable.traverse Data.Traversable.traverse__ GHC.Base.Applicative
      GHC.Base.Functor GHC.Base.Monad GHC.Base.Monoid GHC.Base.Semigroup
      GHC.Base.build' GHC.Base.const GHC.Base.flip GHC.Base.fmap__ GHC.Base.id
