examples/ghc/lib/Pair.v
@@ -40,64 +40,71 @@ Definition pSnd {a} (arg_0__ : Pair a) :=
 (* Converted value declarations: *)
 
 Local Definition Functor__Pair_fmap
-   : forall {a} {b}, (a -> b) -> Pair a -> Pair b :=
-  fun {a} {b} =>
+   : forall {a : Type}, forall {b : Type}, (a -> b) -> Pair a -> Pair b :=
+  fun {a : Type} {b : Type} =>
     fun arg_0__ arg_1__ =>
       match arg_0__, arg_1__ with
       | f, Mk_Pair x y => Mk_Pair (f x) (f y)
       end.
 
 Local Definition Functor__Pair_op_zlzd__
-   : forall {a} {b}, a -> Pair b -> Pair a :=
-  fun {a} {b} => Functor__Pair_fmap GHC.Base.∘ GHC.Base.const.
+   : forall {a : Type}, forall {b : Type}, a -> Pair b -> Pair a :=
+  fun {a : Type} {b : Type} => Functor__Pair_fmap GHC.Base.∘ GHC.Base.const.
 
 Program Instance Functor__Pair : GHC.Base.Functor Pair :=
   fun _ k__ =>
-    k__ {| GHC.Base.fmap__ := fun {a} {b} => Functor__Pair_fmap ;
-           GHC.Base.op_zlzd____ := fun {a} {b} => Functor__Pair_op_zlzd__ |}.
+    k__ {| GHC.Base.fmap__ := fun {a : Type} {b : Type} => Functor__Pair_fmap ;
+           GHC.Base.op_zlzd____ := fun {a : Type} {b : Type} => Functor__Pair_op_zlzd__ |}.
 
 Local Definition Applicative__Pair_op_zlztzg__
-   : forall {a} {b}, Pair (a -> b) -> Pair a -> Pair b :=
-  fun {a} {b} =>
+   : forall {a : Type}, forall {b : Type}, Pair (a -> b) -> Pair a -> Pair b :=
+  fun {a : Type} {b : Type} =>
     fun arg_0__ arg_1__ =>
       match arg_0__, arg_1__ with
       | Mk_Pair f g, Mk_Pair x y => Mk_Pair (f x) (g y)
       end.
 
 Local Definition Applicative__Pair_liftA2
-   : forall {a} {b} {c}, (a -> b -> c) -> Pair a -> Pair b -> Pair c :=
-  fun {a} {b} {c} => fun f x => Applicative__Pair_op_zlztzg__ (GHC.Base.fmap f x).
+   : forall {a : Type},
+     forall {b : Type},
+     forall {c : Type}, (a -> b -> c) -> Pair a -> Pair b -> Pair c :=
+  fun {a : Type} {b : Type} {c : Type} =>
+    fun f x => Applicative__Pair_op_zlztzg__ (GHC.Base.fmap f x).
 
 Local Definition Applicative__Pair_op_ztzg__
-   : forall {a} {b}, Pair a -> Pair b -> Pair b :=
-  fun {a} {b} =>
+   : forall {a : Type}, forall {b : Type}, Pair a -> Pair b -> Pair b :=
+  fun {a : Type} {b : Type} =>
     fun a1 a2 => Applicative__Pair_op_zlztzg__ (GHC.Base.id GHC.Base.<$ a1) a2.
 
-Local Definition Applicative__Pair_pure : forall {a}, a -> Pair a :=
-  fun {a} => fun x => Mk_Pair x x.
+Local Definition Applicative__Pair_pure : forall {a : Type}, a -> Pair a :=
+  fun {a : Type} => fun x => Mk_Pair x x.
 
 Program Instance Applicative__Pair : GHC.Base.Applicative Pair :=
   fun _ k__ =>
-    k__ {| GHC.Base.liftA2__ := fun {a} {b} {c} => Applicative__Pair_liftA2 ;
-           GHC.Base.op_zlztzg____ := fun {a} {b} => Applicative__Pair_op_zlztzg__ ;
-           GHC.Base.op_ztzg____ := fun {a} {b} => Applicative__Pair_op_ztzg__ ;
-           GHC.Base.pure__ := fun {a} => Applicative__Pair_pure |}.
+    k__ {| GHC.Base.liftA2__ := fun {a : Type} {b : Type} {c : Type} =>
+             Applicative__Pair_liftA2 ;
+           GHC.Base.op_zlztzg____ := fun {a : Type} {b : Type} =>
+             Applicative__Pair_op_zlztzg__ ;
+           GHC.Base.op_ztzg____ := fun {a : Type} {b : Type} =>
+             Applicative__Pair_op_ztzg__ ;
+           GHC.Base.pure__ := fun {a : Type} => Applicative__Pair_pure |}.
 
 Local Definition Foldable__Pair_foldMap
-   : forall {m} {a}, forall `{GHC.Base.Monoid m}, (a -> m) -> Pair a -> m :=
-  fun {m} {a} `{GHC.Base.Monoid m} =>
+   : forall {m : Type},
+     forall {a : Type}, forall `{GHC.Base.Monoid m}, (a -> m) -> Pair a -> m :=
+  fun {m : Type} {a : Type} `{GHC.Base.Monoid m} =>
     fun arg_0__ arg_1__ =>
       match arg_0__, arg_1__ with
       | f, Mk_Pair x y => GHC.Base.mappend (f x) (f y)
       end.
 
 Local Definition Foldable__Pair_fold
-   : forall {m}, forall `{GHC.Base.Monoid m}, Pair m -> m :=
-  fun {m} `{GHC.Base.Monoid m} => Foldable__Pair_foldMap GHC.Base.id.
+   : forall {m : Type}, forall `{GHC.Base.Monoid m}, Pair m -> m :=
+  fun {m : Type} `{GHC.Base.Monoid m} => Foldable__Pair_foldMap GHC.Base.id.
 
 Local Definition Foldable__Pair_foldl
-   : forall {b} {a}, (b -> a -> b) -> b -> Pair a -> b :=
-  fun {b} {a} =>
+   : forall {b : Type}, forall {a : Type}, (b -> a -> b) -> b -> Pair a -> b :=
+  fun {b : Type} {a : Type} =>
     fun f z t =>
       Data.SemigroupInternal.appEndo (Data.SemigroupInternal.getDual
                                       (Foldable__Pair_foldMap (Data.SemigroupInternal.Mk_Dual GHC.Base.∘
@@ -105,129 +112,151 @@ Local Definition Foldable__Pair_foldl
                                                                 GHC.Base.flip f)) t)) z.
 
 Local Definition Foldable__Pair_foldr
-   : forall {a} {b}, (a -> b -> b) -> b -> Pair a -> b :=
-  fun {a} {b} =>
+   : forall {a : Type}, forall {b : Type}, (a -> b -> b) -> b -> Pair a -> b :=
+  fun {a : Type} {b : Type} =>
     fun f z t =>
       Data.SemigroupInternal.appEndo (Foldable__Pair_foldMap
                                       (Coq.Program.Basics.compose Data.SemigroupInternal.Mk_Endo f) t) z.
 
 Local Definition Foldable__Pair_foldl'
-   : forall {b} {a}, (b -> a -> b) -> b -> Pair a -> b :=
-  fun {b} {a} =>
+   : forall {b : Type}, forall {a : Type}, (b -> a -> b) -> b -> Pair a -> b :=
+  fun {b : Type} {a : Type} =>
     fun f z0 xs =>
       let f' := fun x k z => k (f z x) in Foldable__Pair_foldr f' GHC.Base.id xs z0.
 
 Local Definition Foldable__Pair_foldr'
-   : forall {a} {b}, (a -> b -> b) -> b -> Pair a -> b :=
-  fun {a} {b} =>
+   : forall {a : Type}, forall {b : Type}, (a -> b -> b) -> b -> Pair a -> b :=
+  fun {a : Type} {b : Type} =>
     fun f z0 xs =>
       let f' := fun k x z => k (f x z) in Foldable__Pair_foldl f' GHC.Base.id xs z0.
 
-Local Definition Foldable__Pair_length : forall {a}, Pair a -> GHC.Num.Int :=
-  fun {a} =>
+Local Definition Foldable__Pair_length
+   : forall {a : Type}, Pair a -> GHC.Num.Int :=
+  fun {a : Type} =>
     Foldable__Pair_foldl' (fun arg_0__ arg_1__ =>
                              match arg_0__, arg_1__ with
                              | c, _ => c GHC.Num.+ #1
                              end) #0.
 
-Local Definition Foldable__Pair_null : forall {a}, Pair a -> bool :=
-  fun {a} => Foldable__Pair_foldr (fun arg_0__ arg_1__ => false) true.
+Local Definition Foldable__Pair_null : forall {a : Type}, Pair a -> bool :=
+  fun {a : Type} => Foldable__Pair_foldr (fun arg_0__ arg_1__ => false) true.
 
 Local Definition Foldable__Pair_product
-   : forall {a}, forall `{GHC.Num.Num a}, Pair a -> a :=
-  fun {a} `{GHC.Num.Num a} =>
+   : forall {a : Type}, forall `{GHC.Num.Num a}, Pair a -> a :=
+  fun {a : Type} `{GHC.Num.Num a} =>
     Coq.Program.Basics.compose Data.SemigroupInternal.getProduct
                                (Foldable__Pair_foldMap Data.SemigroupInternal.Mk_Product).
 
 Local Definition Foldable__Pair_sum
-   : forall {a}, forall `{GHC.Num.Num a}, Pair a -> a :=
-  fun {a} `{GHC.Num.Num a} =>
+   : forall {a : Type}, forall `{GHC.Num.Num a}, Pair a -> a :=
+  fun {a : Type} `{GHC.Num.Num a} =>
     Coq.Program.Basics.compose Data.SemigroupInternal.getSum (Foldable__Pair_foldMap
                                 Data.SemigroupInternal.Mk_Sum).
 
-Local Definition Foldable__Pair_toList : forall {a}, Pair a -> list a :=
-  fun {a} =>
+Local Definition Foldable__Pair_toList : forall {a : Type}, Pair a -> list a :=
+  fun {a : Type} =>
     fun t => GHC.Base.build' (fun _ => (fun c n => Foldable__Pair_foldr c n t)).
 
 Program Instance Foldable__Pair : Data.Foldable.Foldable Pair :=
   fun _ k__ =>
-    k__ {| Data.Foldable.fold__ := fun {m} `{GHC.Base.Monoid m} =>
+    k__ {| Data.Foldable.fold__ := fun {m : Type} `{GHC.Base.Monoid m} =>
              Foldable__Pair_fold ;
-           Data.Foldable.foldMap__ := fun {m} {a} `{GHC.Base.Monoid m} =>
+           Data.Foldable.foldMap__ := fun {m : Type} {a : Type} `{GHC.Base.Monoid m} =>
              Foldable__Pair_foldMap ;
-           Data.Foldable.foldl__ := fun {b} {a} => Foldable__Pair_foldl ;
-           Data.Foldable.foldl'__ := fun {b} {a} => Foldable__Pair_foldl' ;
-           Data.Foldable.foldr__ := fun {a} {b} => Foldable__Pair_foldr ;
-           Data.Foldable.foldr'__ := fun {a} {b} => Foldable__Pair_foldr' ;
-           Data.Foldable.length__ := fun {a} => Foldable__Pair_length ;
-           Data.Foldable.null__ := fun {a} => Foldable__Pair_null ;
-           Data.Foldable.product__ := fun {a} `{GHC.Num.Num a} => Foldable__Pair_product ;
-           Data.Foldable.sum__ := fun {a} `{GHC.Num.Num a} => Foldable__Pair_sum ;
-           Data.Foldable.toList__ := fun {a} => Foldable__Pair_toList |}.
+           Data.Foldable.foldl__ := fun {b : Type} {a : Type} => Foldable__Pair_foldl ;
+           Data.Foldable.foldl'__ := fun {b : Type} {a : Type} => Foldable__Pair_foldl' ;
+           Data.Foldable.foldr__ := fun {a : Type} {b : Type} => Foldable__Pair_foldr ;
+           Data.Foldable.foldr'__ := fun {a : Type} {b : Type} => Foldable__Pair_foldr' ;
+           Data.Foldable.length__ := fun {a : Type} => Foldable__Pair_length ;
+           Data.Foldable.null__ := fun {a : Type} => Foldable__Pair_null ;
+           Data.Foldable.product__ := fun {a : Type} `{GHC.Num.Num a} =>
+             Foldable__Pair_product ;
+           Data.Foldable.sum__ := fun {a : Type} `{GHC.Num.Num a} => Foldable__Pair_sum ;
+           Data.Foldable.toList__ := fun {a : Type} => Foldable__Pair_toList |}.
 
 Local Definition Traversable__Pair_traverse
-   : forall {f} {a} {b},
+   : forall {f : Type -> Type},
+     forall {a : Type},
+     forall {b : Type},
      forall `{GHC.Base.Applicative f}, (a -> f b) -> Pair a -> f (Pair b) :=
-  fun {f} {a} {b} `{GHC.Base.Applicative f} =>
+  fun {f : Type -> Type} {a : Type} {b : Type} `{GHC.Base.Applicative f} =>
     fun arg_0__ arg_1__ =>
       match arg_0__, arg_1__ with
       | f, Mk_Pair x y => (Mk_Pair Data.Functor.<$> f x) GHC.Base.<*> f y
       end.
 
 Local Definition Traversable__Pair_mapM
-   : forall {m} {a} {b},
+   : forall {m : Type -> Type},
+     forall {a : Type},
+     forall {b : Type},
      forall `{GHC.Base.Monad m}, (a -> m b) -> Pair a -> m (Pair b) :=
-  fun {m} {a} {b} `{GHC.Base.Monad m} => Traversable__Pair_traverse.
+  fun {m : Type -> Type} {a : Type} {b : Type} `{GHC.Base.Monad m} =>
+    Traversable__Pair_traverse.
 
 Local Definition Traversable__Pair_sequenceA
-   : forall {f} {a}, forall `{GHC.Base.Applicative f}, Pair (f a) -> f (Pair a) :=
-  fun {f} {a} `{GHC.Base.Applicative f} => Traversable__Pair_traverse GHC.Base.id.
+   : forall {f : Type -> Type},
+     forall {a : Type}, forall `{GHC.Base.Applicative f}, Pair (f a) -> f (Pair a) :=
+  fun {f : Type -> Type} {a : Type} `{GHC.Base.Applicative f} =>
+    Traversable__Pair_traverse GHC.Base.id.
 
 Local Definition Traversable__Pair_sequence
-   : forall {m} {a}, forall `{GHC.Base.Monad m}, Pair (m a) -> m (Pair a) :=
-  fun {m} {a} `{GHC.Base.Monad m} => Traversable__Pair_sequenceA.
+   : forall {m : Type -> Type},
+     forall {a : Type}, forall `{GHC.Base.Monad m}, Pair (m a) -> m (Pair a) :=
+  fun {m : Type -> Type} {a : Type} `{GHC.Base.Monad m} =>
+    Traversable__Pair_sequenceA.
 
 Program Instance Traversable__Pair : Data.Traversable.Traversable Pair :=
   fun _ k__ =>
-    k__ {| Data.Traversable.mapM__ := fun {m} {a} {b} `{GHC.Base.Monad m} =>
+    k__ {| Data.Traversable.mapM__ := fun {m : Type -> Type}
+           {a : Type}
+           {b : Type}
+           `{GHC.Base.Monad m} =>
              Traversable__Pair_mapM ;
-           Data.Traversable.sequence__ := fun {m} {a} `{GHC.Base.Monad m} =>
+           Data.Traversable.sequence__ := fun {m : Type -> Type}
+           {a : Type}
+           `{GHC.Base.Monad m} =>
              Traversable__Pair_sequence ;
-           Data.Traversable.sequenceA__ := fun {f} {a} `{GHC.Base.Applicative f} =>
+           Data.Traversable.sequenceA__ := fun {f : Type -> Type}
+           {a : Type}
+           `{GHC.Base.Applicative f} =>
              Traversable__Pair_sequenceA ;
-           Data.Traversable.traverse__ := fun {f} {a} {b} `{GHC.Base.Applicative f} =>
+           Data.Traversable.traverse__ := fun {f : Type -> Type}
+           {a : Type}
+           {b : Type}
+           `{GHC.Base.Applicative f} =>
              Traversable__Pair_traverse |}.
 
-Local Definition Semigroup__Pair_op_zlzlzgzg__ {inst_a} `{GHC.Base.Semigroup
-  inst_a}
-   : (Pair inst_a) -> (Pair inst_a) -> (Pair inst_a) :=
+Local Definition Semigroup__Pair_op_zlzlzgzg__ {inst_a : Type}
+  `{GHC.Base.Semigroup inst_a}
+   : Pair inst_a -> Pair inst_a -> Pair inst_a :=
   fun arg_0__ arg_1__ =>
     match arg_0__, arg_1__ with
     | Mk_Pair a1 b1, Mk_Pair a2 b2 =>
         Mk_Pair (a1 GHC.Base.<<>> a2) (b1 GHC.Base.<<>> b2)
     end.
 
-Program Instance Semigroup__Pair {a} `{GHC.Base.Semigroup a}
+Program Instance Semigroup__Pair {a : Type} `{GHC.Base.Semigroup a}
    : GHC.Base.Semigroup (Pair a) :=
   fun _ k__ =>
     k__ {| GHC.Base.op_zlzlzgzg____ := Semigroup__Pair_op_zlzlzgzg__ |}.
 
-Local Definition Monoid__Pair_mappend {inst_a} `{GHC.Base.Semigroup inst_a}
-  `{GHC.Base.Monoid inst_a}
-   : (Pair inst_a) -> (Pair inst_a) -> (Pair inst_a) :=
+Local Definition Monoid__Pair_mappend {inst_a : Type} `{GHC.Base.Semigroup
+  inst_a} `{GHC.Base.Monoid inst_a}
+   : Pair inst_a -> Pair inst_a -> Pair inst_a :=
   _GHC.Base.<<>>_.
 
-Local Definition Monoid__Pair_mempty {inst_a} `{GHC.Base.Semigroup inst_a}
-  `{GHC.Base.Monoid inst_a}
-   : (Pair inst_a) :=
+Local Definition Monoid__Pair_mempty {inst_a : Type} `{GHC.Base.Semigroup
+  inst_a} `{GHC.Base.Monoid inst_a}
+   : Pair inst_a :=
   Mk_Pair GHC.Base.mempty GHC.Base.mempty.
 
-Local Definition Monoid__Pair_mconcat {inst_a} `{GHC.Base.Semigroup inst_a}
-  `{GHC.Base.Monoid inst_a}
-   : list (Pair inst_a) -> (Pair inst_a) :=
+Local Definition Monoid__Pair_mconcat {inst_a : Type} `{GHC.Base.Semigroup
+  inst_a} `{GHC.Base.Monoid inst_a}
+   : list (Pair inst_a) -> Pair inst_a :=
   GHC.Base.foldr Monoid__Pair_mappend Monoid__Pair_mempty.
 
-Program Instance Monoid__Pair {a} `{GHC.Base.Semigroup a} `{GHC.Base.Monoid a}
+Program Instance Monoid__Pair {a : Type} `{GHC.Base.Semigroup a}
+  `{GHC.Base.Monoid a}
    : GHC.Base.Monoid (Pair a) :=
   fun _ k__ =>
     k__ {| GHC.Base.mappend__ := Monoid__Pair_mappend ;
@@ -237,29 +266,29 @@ Program Instance Monoid__Pair {a} `{GHC.Base.Semigroup a} `{GHC.Base.Monoid a}
 (* Skipping all instances of class `Outputable.Outputable', including
    `Pair.Outputable__Pair' *)
 
-Definition unPair {a} : Pair a -> (a * a)%type :=
+Definition unPair {a : Type} : Pair a -> (a * a)%type :=
   fun '(Mk_Pair x y) => pair x y.
 
-Definition toPair {a} : (a * a)%type -> Pair a :=
+Definition toPair {a : Type} : (a * a)%type -> Pair a :=
   fun '(pair x y) => Mk_Pair x y.
 
-Definition swap {a} : Pair a -> Pair a :=
+Definition swap {a : Type} : Pair a -> Pair a :=
   fun '(Mk_Pair x y) => Mk_Pair y x.
 
-Definition pLiftFst {a} : (a -> a) -> Pair a -> Pair a :=
+Definition pLiftFst {a : Type} : (a -> a) -> Pair a -> Pair a :=
   fun arg_0__ arg_1__ =>
     match arg_0__, arg_1__ with
     | f, Mk_Pair a b => Mk_Pair (f a) b
     end.
 
-Definition pLiftSnd {a} : (a -> a) -> Pair a -> Pair a :=
+Definition pLiftSnd {a : Type} : (a -> a) -> Pair a -> Pair a :=
   fun arg_0__ arg_1__ =>
     match arg_0__, arg_1__ with
     | f, Mk_Pair a b => Mk_Pair a (f b)
     end.
 
 (* External variables:
-     bool false list op_zt__ pair true Coq.Program.Basics.compose
+     Type bool false list op_zt__ pair true Coq.Program.Basics.compose
      Data.Foldable.Foldable Data.Foldable.foldMap__ Data.Foldable.fold__
      Data.Foldable.foldl'__ Data.Foldable.foldl__ Data.Foldable.foldr'__
      Data.Foldable.foldr__ Data.Foldable.length__ Data.Foldable.null__
