examples/ghc/lib/DynFlags.v
@@ -20,6 +20,7 @@ Require GHC.Base.
 Require GHC.Char.
 Require GHC.Err.
 Require GHC.Num.
+Require GHC.Tuple.
 Require Module.
 Require SrcLoc.
 
@@ -388,10 +389,10 @@ Inductive DynLibLoader : Type :=
 
 Axiom DynFlags : Type.
 
-Record HasDynFlags__Dict m := HasDynFlags__Dict_Build {
+Record HasDynFlags__Dict (m : Type -> Type) := HasDynFlags__Dict_Build {
   getDynFlags__ : m DynFlags }.
 
-Definition HasDynFlags m :=
+Definition HasDynFlags (m : Type -> Type) :=
   forall r__, (HasDynFlags__Dict m -> r__) -> r__.
 Existing Class HasDynFlags.
 
@@ -485,10 +486,10 @@ Inductive Deprecation : Type :=
   | NotDeprecated : Deprecation
   | Deprecated : Deprecation.
 
-Record ContainsDynFlags__Dict t := ContainsDynFlags__Dict_Build {
+Record ContainsDynFlags__Dict (t : Type) := ContainsDynFlags__Dict_Build {
   extractDynFlags__ : t -> DynFlags }.
 
-Definition ContainsDynFlags t :=
+Definition ContainsDynFlags (t : Type) :=
   forall r__, (ContainsDynFlags__Dict t -> r__) -> r__.
 Existing Class ContainsDynFlags.
 
@@ -1273,16 +1274,14 @@ Axiom safeImplicitImpsReq : DynFlags -> bool.
 
 (* Skipping definition `DynFlags.combineSafeFlags' *)
 
-Axiom unsafeFlags : list (GHC.Base.String * (DynFlags -> SrcLoc.SrcSpan) *
-                          (DynFlags -> bool) *
-                          (DynFlags -> DynFlags))%type.
+Axiom unsafeFlags : list (GHC.Tuple.quad_type GHC.Base.String (DynFlags ->
+                                               SrcLoc.SrcSpan) (DynFlags -> bool) (DynFlags -> DynFlags)).
 
-Axiom unsafeFlagsForInfer : list (GHC.Base.String * (DynFlags -> SrcLoc.SrcSpan)
-                                  *
-                                  (DynFlags -> bool) *
-                                  (DynFlags -> DynFlags))%type.
+Axiom unsafeFlagsForInfer : list (GHC.Tuple.quad_type GHC.Base.String
+                                                      (DynFlags -> SrcLoc.SrcSpan) (DynFlags -> bool) (DynFlags ->
+                                                       DynFlags)).
 
-Axiom getOpts : forall {a}, DynFlags -> (DynFlags -> list a) -> list a.
+Axiom getOpts : forall {a : Type}, DynFlags -> (DynFlags -> list a) -> list a.
 
 Axiom getVerbFlags : DynFlags -> list GHC.Base.String.
 
@@ -1750,6 +1749,6 @@ Axiom emptyFilesToClean : FilesToClean.
      Type bool list op_zt__ option BinNums.N Data.Either.Either
      Data.Set.Internal.Set_ EnumSet.EnumSet GHC.Base.Eq_ GHC.Base.Ord GHC.Base.String
      GHC.Char.Char GHC.Err.Build_Default GHC.Err.Default GHC.Err.default
-     GHC.Num.Integer Module.ComponentId Module.Module Module.ModuleName Module.UnitId
-     SrcLoc.Located SrcLoc.SrcSpan
+     GHC.Num.Integer GHC.Tuple.quad_type Module.ComponentId Module.Module
+     Module.ModuleName Module.UnitId SrcLoc.Located SrcLoc.SrcSpan
 *)
