examples/ghc/lib/NameEnv.v
@@ -29,96 +29,101 @@ Definition DNameEnv :=
 
 (* Skipping definition `NameEnv.depAnal' *)
 
-Definition nameEnvElts {a} : NameEnv a -> list a :=
+Definition nameEnvElts {a : Type} : NameEnv a -> list a :=
   fun x => UniqFM.eltsUFM x.
 
-Definition emptyNameEnv {a} : NameEnv a :=
+Definition emptyNameEnv {a : Type} : NameEnv a :=
   UniqFM.emptyUFM.
 
-Definition isEmptyNameEnv {a} : NameEnv a -> bool :=
+Definition isEmptyNameEnv {a : Type} : NameEnv a -> bool :=
   UniqFM.isNullUFM.
 
-Definition unitNameEnv {a} : Name.Name -> a -> NameEnv a :=
+Definition unitNameEnv {a : Type} : Name.Name -> a -> NameEnv a :=
   fun x y => UniqFM.unitUFM x y.
 
-Definition extendNameEnv {a} : NameEnv a -> Name.Name -> a -> NameEnv a :=
+Definition extendNameEnv {a : Type}
+   : NameEnv a -> Name.Name -> a -> NameEnv a :=
   fun x y z => UniqFM.addToUFM x y z.
 
-Definition extendNameEnvList {a}
+Definition extendNameEnvList {a : Type}
    : NameEnv a -> list (Name.Name * a)%type -> NameEnv a :=
   fun x l => UniqFM.addListToUFM x l.
 
-Definition lookupNameEnv {a} : NameEnv a -> Name.Name -> option a :=
+Definition lookupNameEnv {a : Type} : NameEnv a -> Name.Name -> option a :=
   fun x y => UniqFM.lookupUFM x y.
 
-Definition alterNameEnv {a}
+Definition alterNameEnv {a : Type}
    : (option a -> option a) -> NameEnv a -> Name.Name -> NameEnv a :=
   UniqFM.alterUFM.
 
-Definition mkNameEnv {a} : list (Name.Name * a)%type -> NameEnv a :=
+Definition mkNameEnv {a : Type} : list (Name.Name * a)%type -> NameEnv a :=
   fun l => UniqFM.listToUFM l.
 
-Definition elemNameEnv {a} : Name.Name -> NameEnv a -> bool :=
+Definition elemNameEnv {a : Type} : Name.Name -> NameEnv a -> bool :=
   fun x y => UniqFM.elemUFM x y.
 
-Definition plusNameEnv {a} : NameEnv a -> NameEnv a -> NameEnv a :=
+Definition plusNameEnv {a : Type} : NameEnv a -> NameEnv a -> NameEnv a :=
   fun x y => UniqFM.plusUFM x y.
 
-Definition plusNameEnv_C {a}
+Definition plusNameEnv_C {a : Type}
    : (a -> a -> a) -> NameEnv a -> NameEnv a -> NameEnv a :=
   fun f x y => UniqFM.plusUFM_C f x y.
 
-Definition extendNameEnv_C {a}
+Definition extendNameEnv_C {a : Type}
    : (a -> a -> a) -> NameEnv a -> Name.Name -> a -> NameEnv a :=
   fun f x y z => UniqFM.addToUFM_C f x y z.
 
-Definition mapNameEnv {elt1} {elt2}
+Definition mapNameEnv {elt1 : Type} {elt2 : Type}
    : (elt1 -> elt2) -> NameEnv elt1 -> NameEnv elt2 :=
   fun f x => UniqFM.mapUFM f x.
 
-Definition extendNameEnv_Acc {a} {b}
+Definition extendNameEnv_Acc {a : Type} {b : Type}
    : (a -> b -> b) -> (a -> b) -> NameEnv b -> Name.Name -> a -> NameEnv b :=
   fun x y z a b => UniqFM.addToUFM_Acc x y z a b.
 
-Definition extendNameEnvList_C {a}
+Definition extendNameEnvList_C {a : Type}
    : (a -> a -> a) -> NameEnv a -> list (Name.Name * a)%type -> NameEnv a :=
   fun x y z => UniqFM.addListToUFM_C x y z.
 
-Definition delFromNameEnv {a} : NameEnv a -> Name.Name -> NameEnv a :=
+Definition delFromNameEnv {a : Type} : NameEnv a -> Name.Name -> NameEnv a :=
   fun x y => UniqFM.delFromUFM x y.
 
-Definition delListFromNameEnv {a} : NameEnv a -> list Name.Name -> NameEnv a :=
+Definition delListFromNameEnv {a : Type}
+   : NameEnv a -> list Name.Name -> NameEnv a :=
   fun x y => UniqFM.delListFromUFM x y.
 
-Definition filterNameEnv {elt} : (elt -> bool) -> NameEnv elt -> NameEnv elt :=
+Definition filterNameEnv {elt : Type}
+   : (elt -> bool) -> NameEnv elt -> NameEnv elt :=
   fun x y => UniqFM.filterUFM x y.
 
-Definition anyNameEnv {elt} : (elt -> bool) -> NameEnv elt -> bool :=
+Definition anyNameEnv {elt : Type} : (elt -> bool) -> NameEnv elt -> bool :=
   fun f x => UniqFM.foldUFM (orb GHC.Base.∘ f) false x.
 
-Definition disjointNameEnv {a} : NameEnv a -> NameEnv a -> bool :=
+Definition disjointNameEnv {a : Type} : NameEnv a -> NameEnv a -> bool :=
   fun x y => UniqFM.isNullUFM (UniqFM.intersectUFM x y).
 
 (* Skipping definition `NameEnv.lookupNameEnv_NF' *)
 
-Definition emptyDNameEnv {a} : DNameEnv a :=
+Definition emptyDNameEnv {a : Type} : DNameEnv a :=
   UniqFM.emptyUFM.
 
-Definition lookupDNameEnv {a} : DNameEnv a -> Name.Name -> option a :=
+Definition lookupDNameEnv {a : Type} : DNameEnv a -> Name.Name -> option a :=
   UniqFM.lookupUFM.
 
-Definition mapDNameEnv {a} {b} : (a -> b) -> DNameEnv a -> DNameEnv b :=
+Definition mapDNameEnv {a : Type} {b : Type}
+   : (a -> b) -> DNameEnv a -> DNameEnv b :=
   UniqFM.mapUFM.
 
-Definition alterDNameEnv {a}
+Definition alterDNameEnv {a : Type}
    : (option a -> option a) -> DNameEnv a -> Name.Name -> DNameEnv a :=
   UniqFM.alterUFM.
 
 (* External variables:
-     bool false list op_zt__ option orb GHC.Base.op_z2218U__ Name.Name UniqFM.UniqFM
-     UniqFM.addListToUFM UniqFM.addListToUFM_C UniqFM.addToUFM UniqFM.addToUFM_Acc
-     UniqFM.addToUFM_C UniqFM.alterUFM UniqFM.delFromUFM UniqFM.delListFromUFM
-     UniqFM.elemUFM UniqFM.eltsUFM UniqFM.emptyUFM UniqFM.filterUFM UniqFM.foldUFM
-     UniqFM.intersectUFM UniqFM.isNullUFM UniqFM.listToUFM UniqFM.lookupUFM
-     UniqFM.mapUFM UniqFM.plusUFM UniqFM.plusUFM_C UniqFM.unitUFM
+     Type bool false list op_zt__ option orb GHC.Base.op_z2218U__ Name.Name
+     UniqFM.UniqFM UniqFM.addListToUFM UniqFM.addListToUFM_C UniqFM.addToUFM
+     UniqFM.addToUFM_Acc UniqFM.addToUFM_C UniqFM.alterUFM UniqFM.delFromUFM
+     UniqFM.delListFromUFM UniqFM.elemUFM UniqFM.eltsUFM UniqFM.emptyUFM
+     UniqFM.filterUFM UniqFM.foldUFM UniqFM.intersectUFM UniqFM.isNullUFM
+     UniqFM.listToUFM UniqFM.lookupUFM UniqFM.mapUFM UniqFM.plusUFM UniqFM.plusUFM_C
+     UniqFM.unitUFM
 *)
